pulse/src/checker/Pulse.Checker.AssertWithBinders.fst
@@ -406,7 +406,7 @@ let check
     let (| uvs, v_opened, body_opened |) = open_binders g bs (mk_env (fstar_env g)) v body in
     let v, body = v_opened, body_opened in
     let (| v, d |) = PC.check_vprop (push_env g uvs) v in
-    let (| g1, nts, _, pre', k_frame |) = Prover.prove pre_typing uvs d in
+    let (| g1, nts, _, pre', k_frame |) = Prover.prove false pre_typing uvs d in
     //
     // No need to check effect labels for the uvs solution here,
     //   since we are checking the substituted body anyway,
