pulse/src/checker/Pulse.Checker.Prover.Explode.fst
@@ -1,0 +1,83 @@
+(*
+   Copyright 2023 Microsoft Research
+
+   Licensed under the Apache License, Version 2.0 (the "License");
+   you may not use this file except in compliance with the License.
+   You may obtain a copy of the License at
+
+       http://www.apache.org/licenses/LICENSE-2.0
+
+   Unless required by applicable law or agreed to in writing, software
+   distributed under the License is distributed on an "AS IS" BASIS,
+   WITHOUT WARRANTIES OR CONDITIONS OF ANY KIND, either express or implied.
+   See the License for the specific language governing permissions and
+   limitations under the License.
+*)
+
+module Pulse.Checker.Prover.Explode
+
+module T = FStar.Tactics
+
+open Pulse.Syntax
+open Pulse.Typing
+open Pulse.PP
+
+open Pulse.Checker.Base
+open Pulse.Checker.Prover.Base
+open Pulse.Typing.Combinators
+
+let has_structure (q:vprop) : bool =
+  match inspect_term q with
+  // | Tm_Pure _
+  | Tm_Star _ _
+  // | Tm_ExistsSL _ _ _
+  -> true
+  | _ -> false
+  
+let explode1
+  (#preamble:_)
+  (pst:prover_state preamble)
+  (q:vprop)
+: T.Tac (option (qs: list vprop & vprop_equiv (push_env pst.pg pst.uvs) (list_as_vprop qs) q))
+=
+  let q_ss = pst.ss.(q) in
+  // info_doc pst.pg None [
+  //   text "Trying to explode" ^/^ pp q_ss;
+  //   text "pst.ss = " ^/^ pp pst.ss;
+  //   text "pst.uvs = " ^/^ pp pst.uvs;
+  //   text "q= " ^/^ pp q;
+  //   text "q_ss= " ^/^ pp q_ss;
+  // ];
+  if has_structure q_ss
+  then (
+    info_doc pst.pg None [
+      text "Exploding" ^/^ pp q_ss;
+      text "into" ^/^ pp (vprop_as_list q_ss);
+    ];
+    Some (| vprop_as_list q_ss, magic () |)
+  ) else None
+
+let rec explode_aux
+  (#preamble:_)
+  (pst:prover_state preamble)
+  (acc : list vprop) (todo : list vprop) : T.Tac (list vprop)
+=
+  match todo with
+  | [] -> acc
+  | q::qs ->
+    let acc = acc @ (match explode1 pst q with | Some (|qs, _|) -> qs | None -> [q]) in
+    explode_aux pst acc qs
+
+let explode
+  (#preamble:_) (pst:prover_state preamble)
+: T.Tac (pst':prover_state preamble {pst' `pst_extends` pst})
+=
+  let remaining_ctxt = explode_aux pst [] pst.remaining_ctxt in
+  let unsolved' = explode_aux pst [] pst.unsolved in
+  { pst with
+    unsolved = unsolved';
+    goals_inv = magic();
+    remaining_ctxt = remaining_ctxt;
+    remaining_ctxt_frame_typing = magic();
+    k = (admit(); pst.k);
+  }
