pulse/src/checker/Pulse.Checker.Prover.Match.Base.fst
@@ -1,0 +1,267 @@
+(*
+   Copyright 2023 Microsoft Research
+
+   Licensed under the Apache License, Version 2.0 (the "License");
+   you may not use this file except in compliance with the License.
+   You may obtain a copy of the License at
+
+       http://www.apache.org/licenses/LICENSE-2.0
+
+   Unless required by applicable law or agreed to in writing, software
+   distributed under the License is distributed on an "AS IS" BASIS,
+   WITHOUT WARRANTIES OR CONDITIONS OF ANY KIND, either express or implied.
+   See the License for the specific language governing permissions and
+   limitations under the License.
+*)
+
+module Pulse.Checker.Prover.Match.Base
+
+open FStar.Tactics.V2
+open FStar.List.Tot
+open FStar.Ghost
+
+open Pulse.Syntax
+open Pulse.Typing
+open Pulse.Typing.Combinators
+open Pulse.Checker.Base
+open Pulse.Checker.Prover.Base
+open Pulse.PP
+
+module RU = Pulse.RuntimeUtils
+module T  = FStar.Tactics.V2
+module P = Pulse.Syntax.Printer
+module PS = Pulse.Checker.Prover.Substs
+
+let vprop_list_equiv_refl (g:env) (vs:list vprop) : vprop_list_equiv g vs vs = admit()
+let vprop_list_equiv_append (g:env) (vs1 vs2 vs3 vs4 : list vprop)
+  (d1 : vprop_list_equiv g vs1 vs2)
+  (d2 : vprop_list_equiv g vs3 vs4)
+  : vprop_list_equiv g (vs1 @ vs3) (vs2 @ vs4)
+  = admit()
+let vprop_list_equiv_trans (g:env) (vs1 vs2 vs3 : list vprop)
+  (d1 : vprop_list_equiv g vs1 vs2)
+  (d2 : vprop_list_equiv g vs2 vs3)
+  : vprop_list_equiv g vs1 vs3
+  = admit()
+let vprop_list_equiv_assoc_l (g:env) (vs1 vs2 vs3 : list vprop)
+  : vprop_list_equiv g (vs1 @ (vs2 @ vs3)) ((vs1 @ vs2) @ vs3)
+  = admit()
+let vprop_list_equiv_assoc_r (g:env) (vs1 vs2 vs3 : list vprop)
+  : vprop_list_equiv g ((vs1 @ vs2) @ vs3) (vs1 @ (vs2 @ vs3))
+  = admit()
+let vprop_list_equiv_elim_append (g:env) (vs1 vs2 : list vprop)
+  : vprop_equiv g (list_as_vprop (vs1 @ vs2)) (list_as_vprop vs1 * list_as_vprop vs2)
+  = admit()
+let vprop_list_equiv_elim_append' (g:env) (vs1 vs2 : list vprop)
+  : vprop_equiv g (list_as_vprop (vs1 @ vs2)) (list_as_vprop vs2 * list_as_vprop vs1)
+  = admit()
+
+(* local aliases *)
+let (>>>) #g #t0 #t1 #t2 = VE_Trans g t0 t1 t2
+let (>>*) #g #t0 #t1 #t2 = vprop_list_equiv_trans g t0 t1 t2
+let cong_r #g #t0 #t1 #t2 (d : vprop_equiv g t1 t2) : vprop_equiv g (t0 * t1) (t0 * t2) =
+  VE_Ctxt _ _ _ _ _ (VE_Refl _ _) d
+let cong_l #g #t0 #t1 #t2 (d : vprop_equiv g t1 t2) : vprop_equiv g (t1 * t0) (t2 * t0) =
+  VE_Ctxt _ _ _ _ _ d (VE_Refl _ _)
+let ve_refl_pf (#g:env) (p q : vprop) (s : squash (p == q)) : vprop_equiv g p q = VE_Refl g p
+
+(* MORE LEMMAS *)
+
+(* This is not trivial since list_as_vprop distinguishes the singleton case...
+maybe it should not? *)
+let list_as_vprop_cons_equiv 
+  (g : env)
+  (p : vprop)
+  (ps : list vprop)
+  : vprop_equiv g (list_as_vprop (p::ps)) (p * list_as_vprop ps)
+= match ps with
+  | [] ->
+    let pf : vprop_equiv g p (p * tm_emp) =
+      VE_Sym _ _ _ (VE_Unit _ _) >>> VE_Comm _ _ _
+    in
+    pf
+  | _  -> VE_Refl _ _
+
+let vprop_list_equiv_cons g p q ps qs d1 d2 =
+  list_as_vprop_cons_equiv g p ps >>>
+  VE_Ctxt _ _ _ _ _ d1 d2 >>>
+  VE_Sym _ _ _ (list_as_vprop_cons_equiv g q qs)
+
+let star_flip g p q r =
+  VE_Assoc _ _ _ _ >>>
+  VE_Ctxt _ _ _ _ _ (VE_Comm _ _ _) (VE_Refl _ _) >>>
+  VE_Sym _ _ _ (VE_Assoc _ _ _ _)
+
+let vprop_list_equiv_flip g p q ps =
+  VE_Ctxt _ _ _ _ _ (VE_Refl _ _) (list_as_vprop_cons_equiv g q ps) >>>
+  star_flip _ _ _ _ >>>
+  VE_Ctxt _ _ _ _ _ (VE_Refl _ _) (VE_Sym _ _ _ <| list_as_vprop_cons_equiv g p ps)
+
+let vprop_list_equiv_push_append g p ps qs = admit()
+
+let vprop_list_equiv_append_r g ps qs rs pf = vprop_list_equiv_append _ _ _ _ _ (VE_Refl _ _) pf
+
+let subst_append ss ps qs =
+  List.Tot.Properties.map_append
+    (fun t -> PS.ss_term t ss)
+    ps qs
+
+let subst_append_equiv g ss ps qs =
+  subst_append ss ps qs;
+  VE_Refl _ _
+
+let subst_list_as_vprop = admit()
+
+(* Is this somewhere else? *)
+let subst_star ss p q = admit()
+(* Compose two match pass results. *)
+let compose_mpr (g:env) (ss : PS.ss_t) (ctxt0 unsolved0 ctxt1 unsolved1 : list vprop)
+  (mpr1 : match_pass_result g ss ctxt0 unsolved0)
+  (mpr2 : match_pass_result g mpr1.ss' mpr1.ctxt1 mpr1.unsolved1)
+  : match_pass_result g ss ctxt0 unsolved0
+= { ss' = mpr2.ss';
+
+    ctxt_matched = mpr1.ctxt_matched @ mpr2.ctxt_matched;
+    ctxt1        = mpr2.ctxt1;
+    ctxt_ok      = 
+      (* quite brittle to write these proofs. *)
+      mpr1.ctxt_ok >>*
+      (vprop_list_equiv_append _ _ _ _ _ (vprop_list_equiv_refl _ _) mpr2.ctxt_ok) >>*
+      (vprop_list_equiv_assoc_l _ _ _ _)
+    ;
+    
+    unsolved_matched = mpr1.unsolved_matched @ mpr2.unsolved_matched;
+    unsolved1 = mpr2.unsolved1;
+    unsolved_ok = (
+      subst_append ss mpr1.unsolved_matched mpr2.unsolved_matched; (* lemma call *)
+      (* proof: *)
+      mpr1.unsolved_ok >>*
+      (vprop_list_equiv_append _ _ _ _ _ (vprop_list_equiv_refl _ _) mpr2.unsolved_ok) >>*
+      (vprop_list_equiv_assoc_l _ _ _ _)
+    );
+
+    match_ok = (
+      assume (mpr1.ss' $$ mpr1.unsolved_matched == mpr2.ss' $$ mpr1.unsolved_matched);
+      (* ^ should hold since mpr1.ss' fully defines the variables in unsolved_matched *)
+      vprop_list_equiv_append _ _ _ _ _ mpr1.match_ok mpr2.match_ok >>*
+      // VE_Sym _ _ _ (subst_append_equiv _ _ _ _) >>*
+      vprop_list_equiv_append _ _ _ _ _
+        (ve_refl_pf #g
+           (list_as_vprop <| (mpr1.ss' $$ mpr1.unsolved_matched))
+           (list_as_vprop <| (mpr2.ss' $$ mpr1.unsolved_matched))
+           ()) (* relies on assumption above *)
+        (VE_Refl _ _)
+      >>* VE_Sym _ _ _ (subst_append_equiv _ _ _ _)
+    );
+  }
+
+let apply_mpr_vequiv_proof
+  (#preamble:_) (pst:prover_state preamble)
+  (mpr : mpr_t pst)
+  : vprop_equiv (push_env pst.pg pst.uvs)
+                ((list_as_vprop pst.remaining_ctxt * preamble.frame) * (mpr.ss'.(pst.solved)))
+                ((list_as_vprop mpr.ctxt1 * preamble.frame) * (mpr.ss'.(list_as_vprop mpr.unsolved_matched * pst.solved)))
+=
+  let pf0 : vprop_equiv (push_env pst.pg pst.uvs)
+             (list_as_vprop pst.remaining_ctxt)
+             (list_as_vprop mpr.ctxt_matched * list_as_vprop mpr.ctxt1)
+  = mpr.ctxt_ok >>>
+    vprop_list_equiv_elim_append _ _ _
+  in
+  let pf1 : vprop_equiv (push_env pst.pg pst.uvs)
+             (list_as_vprop mpr.ctxt_matched * list_as_vprop mpr.ctxt1)
+             (list_as_vprop mpr.ctxt1 * (mpr.ss'.(list_as_vprop mpr.unsolved_matched)))
+  = subst_list_as_vprop mpr.ss' mpr.unsolved_matched;
+    VE_Comm _ _ _ >>>
+    VE_Ctxt _ _ _ _ _ (VE_Refl _ _) mpr.match_ok
+  in
+  let pf2 : vprop_equiv (push_env pst.pg pst.uvs)
+             ((list_as_vprop pst.remaining_ctxt * preamble.frame) * (mpr.ss'.(pst.solved)))
+             ((list_as_vprop mpr.ctxt1 * (mpr.ss'.(list_as_vprop mpr.unsolved_matched) * preamble.frame)) * (mpr.ss'.(pst.solved)))
+  = cong_l (cong_l (pf0 >>> pf1)) >>>
+    cong_l (VE_Sym _ _ _ (VE_Assoc _ _ _ _))
+  in
+  let eq : squash ((mpr.ss'.(list_as_vprop mpr.unsolved_matched) * mpr.ss'.(pst.solved))
+                    ==
+                   mpr.ss'.(list_as_vprop mpr.unsolved_matched * pst.solved))
+  = subst_star mpr.ss' (list_as_vprop mpr.unsolved_matched) pst.solved;
+    ()
+  in
+  let pf3 : vprop_equiv (push_env pst.pg pst.uvs)
+             ((list_as_vprop mpr.ctxt1 * (mpr.ss'.(list_as_vprop mpr.unsolved_matched) * preamble.frame)) * (mpr.ss'.(pst.solved)))
+             ((list_as_vprop mpr.ctxt1 * preamble.frame) * (mpr.ss'.(list_as_vprop mpr.unsolved_matched * pst.solved)))
+  = 
+    FStar.Pure.BreakVC.break_vc ();
+    // ^ this line seems to make the proof much faster
+    // and more reliable, and work without splitting!
+    VE_Sym _ _ _ (VE_Assoc _ _ _ _) >>>
+    cong_r (
+      cong_l (VE_Comm _ _ _) >>>
+      VE_Sym _ _ _ (VE_Assoc _ _ _ _) >>>
+      cong_r (ve_refl_pf ((mpr.ss'.(list_as_vprop mpr.unsolved_matched)) * mpr.ss'.(pst.solved))
+                         (mpr.ss'.(list_as_vprop mpr.unsolved_matched * pst.solved))
+                         eq)
+    ) >>>
+    VE_Assoc _ _ _ _
+  in
+  pf2 >>> pf3
+
+(* Apply a match pass result to the prover state. *)
+let apply_mpr
+  (#preamble:_) (pst:prover_state preamble)
+  (mpr : mpr_t pst)
+  : T.Tac (pst':prover_state preamble { pst' `pst_extends` pst })
+= { pst with
+      pg  = pst.pg;
+      uvs = pst.uvs;
+      ss  = mpr.ss';
+      
+      nts = None; (* Clear substitution cache *)
+ 
+      remaining_ctxt = mpr.ctxt1;
+      remaining_ctxt_frame_typing = RU.magic (); (* inversion? otherwise prove *)
+
+      unsolved = mpr.unsolved1;
+      solved   = list_as_vprop mpr.unsolved_matched * pst.solved;
+      solved_inv = RU.magic (); (* freevars *)
+      
+      (* boring proof *)
+      goals_inv =
+          pst.goals_inv >>>
+          (VE_Ctxt _ _ _ _ _
+            (VE_Trans _ _ _ _ mpr.unsolved_ok (vprop_list_equiv_elim_append' _ _ _))
+            (VE_Refl _ _)) >>>
+          (VE_Sym _ _ _ <| VE_Assoc _ _ _ _)
+      ;
+
+      k = (
+        assume (pst.pg == push_env pst.pg pst.uvs); // FIXME!!! Is the environment on the continuation_elaborator right??
+        let k0 : continuation_elaborator
+                   preamble.g0 (preamble.ctxt * preamble.frame) 
+                   pst.pg      ((list_as_vprop pst.remaining_ctxt * preamble.frame) * pst.ss.(pst.solved))
+        = pst.k
+        in
+        let k1 : continuation_elaborator
+                   pst.pg ((list_as_vprop pst.remaining_ctxt * preamble.frame) * pst.ss.(pst.solved))
+                   pst.pg ((list_as_vprop pst.remaining_ctxt * preamble.frame) * mpr.ss'.(pst.solved))
+        = (admit(); k_elab_unit _ _)
+        in
+        let k2 : continuation_elaborator
+                   pst.pg ((list_as_vprop pst.remaining_ctxt * preamble.frame) * mpr.ss'.(pst.solved))
+                   pst.pg ((list_as_vprop mpr.ctxt1          * preamble.frame) * mpr.ss'.(list_as_vprop mpr.unsolved_matched * pst.solved))
+        = k_elab_equiv (k_elab_unit pst.pg ((list_as_vprop pst.remaining_ctxt * preamble.frame) * mpr.ss'.(pst.solved)))
+            (VE_Refl _ _)
+            (apply_mpr_vequiv_proof pst mpr)
+        in
+        let k3 : continuation_elaborator 
+                   preamble.g0 (preamble.ctxt * preamble.frame) 
+                   pst.pg ((list_as_vprop mpr.ctxt1          * preamble.frame) * mpr.ss'.(list_as_vprop mpr.unsolved_matched * pst.solved))
+        = k0 `k_elab_trans` k1 `k_elab_trans` k2
+        in
+        k3
+      );
+
+      (* Set progress=true if we matched something. *)
+      progress = pst.progress || Cons? mpr.ctxt_matched;
+  }
+
